Some code cleanup and refactoring

examples/rel/Setoids.Crypto.PKAE.fst
@@ -10,6 +10,7 @@ open Setoids.Crypto.ODH
 
 module DM = FStar.DependentMap
 
+#set-options "--z3rlimit 350 --max_fuel 0 --max_ifuel 0"
 let pkey n = share n
 let nonce = bytes
 
@@ -17,6 +18,7 @@ let pkae_state n aes = (ae_log #n aes * odh_state n) * key_state n
 
 let pkae_state_rel n aes = ((lo (ae_log #n aes)) ** (lo (odh_state n))) ** (lo (key_state n))
 
+#set-options "--z3rlimit 350 --max_fuel 0 --max_ifuel 1"
 let lift_ae_state #a (#arel:erel a) n aes (f:eff (lo (ae_log #n aes) ** lo (key_state n)) arel)
   : eff (pkae_state_rel n aes) arel
   = fun (t, ((ae_st, odh_st), key_st)) ->
@@ -31,27 +33,26 @@ let lift_odh_state #a (#arel:erel a) n aes (f:eff (lo (odh_state n) ** lo (key_s
       | None, (odh_st', key_st'), t -> None, ((ae_st,odh_st'), key_st'), t
       | Some x, (odh_st', key_st'), t -> Some x, ((ae_st,odh_st'), key_st'), t
 
+#set-options "--z3rlimit 350 --max_fuel 0 --max_ifuel 0"
 let ae_odh_sig n aes = sig_prod (odh_sig n) (ae_sig n aes)
 let ae_odh_module n aes = module_t (ae_odh_sig n aes)
 
 let pkae_gen_t n aes =
   (lo unit)
-  ^--> eff_rel (((hi (ae_log #n aes)) ** (lo (odh_state n))) ** (lo (key_state n))) (lo (share n))
+    ^--> eff_rel (((hi (ae_log #n aes)) ** (lo (odh_state n))) ** (lo (key_state n))) (lo (share n))
 
 let pkae_gen n aes (m:ae_odh_module n aes) : pkae_gen_t n aes
   =
   fun _ ->
-  let odh_gen : gen_dh_t n = get_oracle m (Inl GEN_DH) in
-  lift_odh_state n aes (odh_gen ())
+    let odh_gen : gen_dh_t n = get_oracle m (Inl GEN_DH) in
+    lift_odh_state n aes (odh_gen ())
 
 let pkae_enc_inputs n (aes:ae_scheme n) = quatruple_rel (lo (pkey n)) (lo (pkey n)) (lo nonce) (lo (p:bytes{len p `lte` aes.max_plaintext_length}))
 
 let pkae_enc_t n aes =
   pkae_enc_inputs n aes
-  ^--> eff_rel (pkae_state_rel n aes) (lo bytes)
+    ^--> eff_rel (pkae_state_rel n aes) (lo bytes)
 
-#set-options "--z3rlimit 350 --max_fuel 2 --max_ifuel 4"
-#set-options "--query_stats"
 let pkae_enc n aes (m:ae_odh_module n aes) : pkae_enc_t n aes =
   fun (sender_pk, receiver_pk, nonce, p) ->
     let odh_exp : odh_t n = get_oracle m (Inl ODH) in
@@ -64,37 +65,46 @@ let pkae_dec_inputs n (aes:ae_scheme n) = quatruple_rel (lo (pkey n)) (lo (pkey 
 
 let pkae_dec_t n aes =
   pkae_dec_inputs n aes
-  ^--> eff_rel (pkae_state_rel n aes) (lo (option (p:bytes{len p `lte` aes.max_plaintext_length})))
+    ^--> eff_rel (pkae_state_rel n aes) (option_rel (lo (p:bytes{len p `lte` aes.max_plaintext_length})))
 
 let pkae_dec n aes (m:ae_odh_module n aes) : pkae_dec_t n aes =
   fun (sender_pk, receiver_pk, nonce, c) ->
     let odh_exp : odh_t n = get_oracle m (Inl ODH) in
     let ae_dec : dec_t n aes = get_oracle m (Inr DEC) in
     h <-- lift_odh_state n aes (odh_exp (sender_pk, receiver_pk));
-    p <-- lift_ae_state #(option (p:bytes{len p `lte` aes.max_plaintext_length})) #(lo (option (p:bytes{len p `lte` aes.max_plaintext_length}))) n aes (ae_dec (c,nonce,h));
-    return #(pkae_state n aes) #(option (p:bytes{len p `lte` aes.max_plaintext_length})) #(pkae_state_rel n aes) p
+    p <-- lift_ae_state n aes (ae_dec (c,nonce,h));
+    return p
 
 type pkae_labels =
     | GEN
     | ENC
     | DEC
 
+#set-options "--z3rlimit 350 --max_fuel 0 --max_ifuel 1"
 let pkae_field_types n aes : pkae_labels -> Type =
     function  GEN -> pkae_gen_t n aes
             | ENC -> pkae_enc_t n aes
             | DEC -> pkae_dec_t n aes
 
-// The relations seem to be the problem. I have removed the relations for now.
 let pkae_field_rels n aes : (l:pkae_labels -> erel (pkae_field_types n aes l)) =
   function
-      GEN -> fun _ _ -> True
-    | ENC -> fun _ _ -> True
-    | DEC -> fun _ _ -> True
+      GEN ->
+      arrow
+        (lo unit)
+        (eff_rel (((hi (ae_log #n aes)) ** (lo (odh_state n))) ** (lo (key_state n))) (lo (share n)))
+    | ENC ->
+      arrow
+        (pkae_enc_inputs n aes)
+        (eff_rel (pkae_state_rel n aes) (lo bytes))
+    | DEC ->
+      arrow
+        (pkae_dec_inputs n aes)
+        (eff_rel (pkae_state_rel n aes) (option_rel (lo (p:bytes{len p `lte` aes.max_plaintext_length}))))
 
 let pkae_sig (n:u32) (aes:ae_scheme n) = {
-  labels = pkae_labels;
-  ops = pkae_field_types n aes;
-  rels = pkae_field_rels n aes
+    labels = pkae_labels;
+    ops = pkae_field_types n aes;
+    rels = pkae_field_rels n aes
   }
 
 let pkae_module (n:u32) (aes:ae_scheme n) (m:ae_odh_module n aes) : module_t (pkae_sig n aes) =
@@ -105,7 +115,7 @@ let pkae_module (n:u32) (aes:ae_scheme n) (m:ae_odh_module n aes) : module_t (pk
 
 let pkae_functor (n:u32) (aes:ae_scheme n)
   : functor_t (sig_prod (odh_sig n) (ae_sig n aes)) (pkae_sig n aes)
-  = fun m ->
+  = fun (m:module_t (sig_prod (odh_sig n) (ae_sig n aes))) ->
       pkae_module n aes m
 
 ///     ID_WRITE
@@ -115,9 +125,6 @@ let key0_id_composition n
   : functor_t sig_unit (sig_prod (key_write_sig n) (key_read_sig n)) =
   let id_composition =
     functor_prod_shared_sig
-      (key_sig n)
-      (key_write_sig n)
-      (key_read_sig n)
       (key_write_functor n)
       (key_read_functor n) in
   comp id_composition (KEY.key0_functor n)
@@ -129,9 +136,6 @@ let key1_id_composition n
   : functor_t sig_unit (sig_prod (key_write_sig n) (key_read_sig n)) =
   let id_composition =
     functor_prod_shared_sig
-      (key_sig n)
-      (key_write_sig n)
-      (key_read_sig n)
       (key_write_functor n)
       (key_read_functor n) in
   comp id_composition (KEY.key1_functor n)
@@ -142,10 +146,6 @@ let key1_id_composition n
 let protocol0_composition n aes
   : functor_t (sig_prod (key_write_sig n) (key_read_sig n)) (sig_prod (odh_sig n) (ae_sig n aes)) =
   functor_prod
-    (key_write_sig n)
-    (odh_sig n)
-    (key_read_sig n)
-    (ae_sig n aes)
     (odh_functor n)
     (ae0_functor n aes)
 
@@ -155,10 +155,6 @@ let protocol0_composition n aes
 let protocol1_composition n aes
   : functor_t (sig_prod (key_write_sig n) (key_read_sig n)) (sig_prod (odh_sig n) (ae_sig n aes)) =
   functor_prod
-    (key_write_sig n)
-    (odh_sig n)
-    (key_read_sig n)
-    (ae_sig n aes)
     (odh_functor n)
     (ae1_functor n aes)
 
@@ -180,8 +176,21 @@ let pkae1_composition n aes
 
 /// Proof:
 /// Assumptions:
-/// - (ODH|ID_READ) o KEY_0 = (ODH|ID_READ) o KEY_1
-/// - (ID_WRITE|AE_0) o KEY_1 = (ID_WRITE|AE_1) o KEY_1
-let pkae_proof (n:u32) (aes:ae_scheme n) : Lemma
-  (ensures (eq (fun _ _ -> True) (sum (ae_eps n aes) (odh_eps n)) (pkae0_composition n aes) (pkae1_composition n aes)))
-  = ()
+/// ODH o ID_WRITE            ODH o ID_WRITE
+/// -------------- o KEY_0 =  -------------- o KEY_1
+///    ID_READ                    ID_READ
+
+///    ID_WRITE                     ID_WRITE
+/// ---------------- o KEY_1 =  ---------------- o KEY_1
+///  AE_0 o ID_READ              AE_1 o ID_READ
+///
+/// First step: pull ODH assumption to the right and make sure the result is still equal.
+///         ID     ODH o ID_WRITE
+///  PKAE o ---- o --------------- o KEY_0
+///         AE_0      ID_READ
+///
+/// Goal: Show that we can instantiate an eq instance with pkae0 and pkae1
+let pkae_proof (n:u32) (aes:ae_scheme n) : unit =
+  let step1 = comp (pkae_functor n aes) (comp (functor_prod id_func (ae0_functor n aes)) (odh_game0 n)) in
+  assert(step1 == pkae0_composition n aes);
+  admit()
