examples/rel/Setoids.Crypto.AE.fst
@@ -12,6 +12,7 @@ module DM = FStar.DependentMap
 //AE package
 ////////////////////////////////////////////////////////////////////////////////
 
+#set-options "--z3rlimit 350 --max_fuel 0 --max_ifuel 0"
 noeq type ae_scheme (n:u32) =
   | AES:
   max_plaintext_length: u32 ->
@@ -24,41 +25,25 @@ let ae_log_key = handle*bytes
 let ae_log_value #n (aes:ae_scheme n) = fun (h,nonce) -> option (bytes*p:bytes{len p `lte` aes.max_plaintext_length})
 
 /// Map from nonces to a maps from ciphertext to plaintexts
+/// Should the state be dependent on the AE scheme?
 let ae_log #n (aes:ae_scheme n) =
   DM.t (handle*bytes) (ae_log_value aes)
 
 let ae_log_rel (#n:u32) (aes:ae_scheme n) = lo (ae_log aes)
 
-let combined_state_t #n aes = ae_log #n aes * key_state n
+let combined_state_t n aes = ae_log #n aes * key_state n
+let combined_state_rel n aes = lo (ae_log #n aes) ** lo (key_state n)
 
-/// Is there a nicer way to have a function with mulitple inputs than using nested tuples?
-/// How to use the 'secure information flow' relations again with AE^0 vs AE^1?
-/// AE^0 also depends on the state of the key package.
-/// Is there a way to improve verification performance and/or error messages?
-/// Every AE function takes as additional parameter the module it is composed with.
-/// AE Functor: Function from underlay module to AE sigu32ure
+let enc_inputs n (aes:ae_scheme n) =
+  triple_rel
+    (lo (p:bytes{len p `lte` aes.max_plaintext_length}))
+    (lo bytes)
+    (lo handle)
 
-#set-options "--z3rlimit 50 --max_fuel 1 --max_ifuel 3"
-/// This would be a nice, generic approach, but it's probably a little to complex
-//let multi_rel' (tl:list Type) (rm:DMap.t (n:u32{n < List.Tot.length tl}) (fun i -> rel (List.Tot.index tl i))) (vm0 vm1:DMap.t (n:u32{n < List.Tot.length tl}) (fun i -> List.Tot.index tl i)) =
-//  let logical_and t1 t2 = t1 /\ t2
-//  let iterate_maps (i:u32{i < List.Tot.length tl}) =
-//    let x0 = DMap.sel vm0 i in
-//    let x1 = DMap.sel vm1 i in
-//    let rel = DMap.sel rm i in
-//    x0 `rel` x1
-//  in
-//  //let indices = mapi #Type (fun i _ -> i) tl in
-//  let prop_list = List.Tot.mapi #Type (fun i _ -> iterate_maps i) tl in
-//  admit()
-
-let enc_inputs #n (aes:ae_scheme n) = triple_rel (lo (p:bytes{len p `lte` aes.max_plaintext_length})) (lo bytes) (lo handle)
-
-#set-options "--z3rlimit 350 --max_fuel 2 --max_ifuel 3"
 /// Ideally, refine length of output bytes to be the relevant function of the input bytes. Maybe a lemma?
 let enc_t (n:u32) (aes:ae_scheme n) =
-  enc_inputs aes
-    ^--> eff_rel (ae_log_rel #n aes ** lo (key_state n)) (lo bytes)
+  enc_inputs n aes
+    ^--> eff_rel (combined_state_rel n aes) (lo bytes)
 
 let enc0 (n:u32) (aes:ae_scheme n) (key_module:module_t (key_read_sig n)) : (enc_t n aes) =
   fun (p,nonce,h) ->
@@ -69,20 +54,16 @@ let enc0 (n:u32) (aes:ae_scheme n) (key_module:module_t (key_read_sig n)) : (enc
       raise #(ae_log #n aes*key_state n)
     | None ->
       let k_get : key_get_t n = get_oracle key_module ID_GET in
-      k <-- lift_right #(ae_log #n aes) #(ae_log_rel #n aes) #(key_state n) #((lo (key_state n))) #(key n) #(lo (key n)) (k_get h);
+      k <-- lift_right (k_get h);
       let c = aes.enc p k nonce in
       let ae_st' = DM.upd ae_st (h,nonce) (Some (c,p)) in
       put (ae_st',k_st);;
       return c
 
-
-#reset-options
-#set-options "--z3rlimit 350 --max_fuel 2 --max_ifuel 3"
-#set-options "--query_stats"
 let enc1 (n:u32) (aes:ae_scheme n) (key_module:module_t (key_read_sig n)) : (enc_t n aes) =
   fun (p,nonce,h) ->
     combined_state <-- get ;
-    let ae_st,k_st : ae_log aes*key_state n = combined_state in
+    let ae_st,k_st : combined_state_t n aes = combined_state in
     match DM.sel #ae_log_key #(ae_log_value aes) ae_st (h,nonce) with
     | Some option_map -> // Nonce is not unique
       raise
@@ -90,53 +71,64 @@ let enc1 (n:u32) (aes:ae_scheme n) (key_module:module_t (key_read_sig n)) : (enc
       c <-- sample_multiple (aes.ciphertext_length (len p));
       let ae_st' = DM.upd ae_st (h,nonce) (Some (c,p)) in
       put (ae_st',k_st);;
-      return #(ae_log #n aes*key_state n) #(bytes) #(ae_log_rel #n aes ** (lo (key_state n))) #(lo bytes) c
+      return #_ #(bytes) c
 
-let dec_inputs #n (aes:ae_scheme n) = triple_rel (lo (c:bytes{len c `lte` aes.ciphertext_length aes.max_plaintext_length})) (lo bytes) (lo handle)
+let dec_inputs n (aes:ae_scheme n) =
+  triple_rel
+    (lo (c:bytes{len c `lte` aes.ciphertext_length aes.max_plaintext_length}))
+    (lo bytes)
+    (lo handle)
 
 let dec_t (n:u32) (aes:ae_scheme n) =
-  dec_inputs aes
-  ^--> eff_rel (ae_log_rel #n aes ** lo (key_state n)) (lo (option (p:bytes{len p `lte` aes.max_plaintext_length})))
+  dec_inputs n aes
+    ^--> eff_rel (combined_state_rel n aes) (option_rel (lo (p:bytes{len p `lte` aes.max_plaintext_length})))
 
 let dec0 (n:u32) (aes:ae_scheme n) (key_module:module_t (key_read_sig n)) : (dec_t n aes) =
   fun (c,nonce,h) ->
   combined_state <-- get ;
   let ae_st,k_st = combined_state in
   let k_get : key_get_t n = get_oracle key_module ID_GET in
-  k <-- lift_right #(ae_log #n aes) #(ae_log_rel #n aes) #(key_state n) #((lo (key_state n))) #(key n) #(lo (key n)) (k_get h);
-  return #(combined_state_t #n aes) #_ #(ae_log_rel #n aes ** hi (key_state n)) #(lo (option (p:bytes{len p `lte` aes.max_plaintext_length}))) (aes.dec c k nonce)
+  k <-- lift_right (k_get h);
+  let option_p = aes.dec c k nonce in
+  return option_p
 
 let dec1 (n:u32) (aes:ae_scheme n) (key_module:module_t (key_read_sig n)) : (dec_t n aes) =
   fun (c,nonce,h) ->
   combined_state <-- get ;
-  let ae_st,k_st : ae_log aes*key_state n = combined_state in
+  let ae_st,k_st : combined_state_t n aes = combined_state in
   match DM.sel ae_st (h,nonce) with
   | Some (c',p) -> // Nonce is not unique
     if c = c' then
-      return #(combined_state_t #n aes) (Some p)
+      return (Some p)
     else
       return None
   | None ->
-    return #(combined_state_t #n aes) #_ #(ae_log_rel #n aes ** hi (key_state n)) #(lo (option (p:bytes{len p `lte` aes.max_plaintext_length}))) None
+    return None
 
 type ae_labels =
     | ENC
     | DEC
 
+#set-options "--z3rlimit 350 --max_fuel 0 --max_ifuel 1"
 let ae_field_types n aes : ae_labels -> Type =
     function  ENC -> enc_t n aes
             | DEC -> dec_t n aes
 
-// The relations seem to be the problem. I have removed the relations for now.
 let ae_field_rels n aes : (l:ae_labels -> erel (ae_field_types n aes l)) =
   function
-      ENC -> fun _ _ -> True //arrow (enc_inputs aes) (eff_rel (ae_log_rel #n aes ** lo (key_state n)) (lo bytes))
-    | DEC -> fun _ _ -> True //arrow (dec_inputs aes) (eff_rel (ae_log_rel #n aes ** lo (key_state n)) (lo (option (p:bytes{len p `lte` aes.max_plaintext_length}))))
+      ENC ->
+        arrow
+          (enc_inputs n aes)
+          (eff_rel (combined_state_rel n aes) (lo bytes))
+    | DEC ->
+        arrow
+          (dec_inputs n aes)
+          (eff_rel (combined_state_rel n aes) (option_rel (lo (p:bytes{len p `lte` aes.max_plaintext_length}))))
 
 let ae_sig (n:u32) (aes:ae_scheme n) = {
-  labels = ae_labels;
-  ops = ae_field_types n aes;
-  rels = ae_field_rels n aes
+    labels = ae_labels;
+    ops = ae_field_types n aes;
+    rels = ae_field_rels n aes
   }
 
 let ae0_module (n:u32) (aes:ae_scheme n) (k:module_t (key_read_sig n)) : module_t (ae_sig n aes) =
@@ -163,18 +155,12 @@ let ae1_functor (n:u32) (aes:ae_scheme n)
 let ae0_composition n (aes:ae_scheme n)
   : functor_t (key_sig n) (sig_prod (key_write_sig n) (ae_sig n aes)) =
   functor_prod_shared_sig
-    (key_sig n)
-    (key_write_sig n)
-    (ae_sig n aes)
     (key_write_functor n)
     (comp (ae0_functor n aes) (key_read_functor n))
 
 let ae1_composition n (aes:ae_scheme n)
   : functor_t (key_sig n) (sig_prod (key_write_sig n) (ae_sig n aes)) =
   functor_prod_shared_sig
-    (key_sig n)
-    (key_write_sig n)
-    (ae_sig n aes)
     (key_write_functor n)
     (comp (ae1_functor n aes) (key_read_functor n))
 
@@ -197,7 +183,4 @@ assume val ae_eps: n:u32 -> aes:ae_scheme n -> eps (sig_unit) (sig_prod (key_wri
 let ae_functor_rel n aes : per (functor_t (sig_unit) (sig_prod (key_write_sig n) (ae_sig n aes))) =
   fun funct_a funct_b -> True
 
-/// Questions:
-/// - What would a relation on a functor look like?
-/// - How to instantiate a hypothesis?
-let ae_assumption n aes = eq (ae_functor_rel n aes) (ae_eps n aes) (ae_game0 n aes) (ae_game1 n aes)
+let ae_assumption n aes = Perfect #(sig_unit) #(sig_prod (key_write_sig n) (ae_sig n aes)) #(fun _ _ -> True) (ae_game0 n aes) (ae_game1 n aes) ()
