examples/rel/Setoids.Crypto.KEY.fst
@@ -10,14 +10,13 @@ module DM = FStar.DependentMap
 //KEY package
 ////////////////////////////////////////////////////////////////////////////////
 
+#set-options "--z3rlimit 350 --max_fuel 0 --max_ifuel 0"
 let handle = h:(bytes&bytes){int_of_bytes (fst h) <= int_of_bytes (snd h)}
 
 let key (n:u32) = lbytes32 n
 let key_state (n:u32) = Map.t handle (option bool) & Map.t handle (option (key n))
 
 private let key_state_rel (n:u32) = lo (key_state n)
-
-//let key_eff (n:u32) = eff (key_state_rel n)
 
 let key_set_t (n:u32) = ((lo handle) ** (lo (key n))) ^--> eff_rel (key_state_rel n) (lo handle)
 let key0_set n : key_set_t n =
@@ -86,6 +85,7 @@ type key_labels =
   | SET
   | CSET
 
+#set-options "--z3rlimit 350 --max_fuel 0 --max_ifuel 1"
 let key_field_types n : key_labels -> Type =
     function  GET -> key_get_t n
             | HON -> key_hon_t n
@@ -100,9 +100,9 @@ let key_field_rels n : (k:key_labels -> erel (key_field_types n k)) =
     | CSET -> arrow (lo handle ** lo (key n)) (eff_rel (key_state_rel n) (lo handle))
 
 let key_sig (n:u32) = {
-  labels = key_labels;
-  ops = key_field_types n;
-  rels = key_field_rels n
+    labels = key_labels;
+    ops = key_field_types n;
+    rels = key_field_rels n
   }
 
 let key0_module (n:u32) : module_t (key_sig n) =
@@ -112,8 +112,6 @@ let key0_module (n:u32) : module_t (key_sig n) =
             | SET -> key0_set n
             | CSET -> key_cset n)
 
-#set-options "--z3rlimit 350 --max_fuel 2 --max_ifuel 3"
-#set-options "--query_stats"
 let key1_module (n:u32) : module_t (key_sig n) =
   DM.create #_ #(key_sig n).ops
     (function GET -> key_get n
@@ -137,16 +135,15 @@ let key_read_field_types n : key_read_labels -> Type0 =
            | ID_HON -> key_hon_t n
 
 let key_read_field_rels n : (l:key_read_labels -> erel (key_read_field_types n l)) =
-  function ID_GET -> fun _ _ -> True //arrow (lo handle) (eff_rel ((lo (key_state n))) (lo (key n)))
-         | ID_HON -> fun _ _ -> True //arrow (lo handle) (eff_rel ((lo (key_state n))) (lo bool))
+  function ID_GET -> arrow (lo handle) (eff_rel #(key_state n) #(key n) ((lo (key_state n))) (lo (key n)))
+         | ID_HON -> arrow (lo handle) (eff_rel #(key_state n) #bool ((lo (key_state n))) (lo bool))
 
 let key_read_sig (n:u32) = {
-  labels = key_read_labels;
-  ops = key_read_field_types n;
-  rels = key_read_field_rels n
+    labels = key_read_labels;
+    ops = key_read_field_types n;
+    rels = key_read_field_rels n
   }
 
-#set-options "--z3rlimit 350 --max_fuel 3 --max_ifuel 4"
 let key_read_module (n:u32) (km:module_t (key_sig n)) : module_t (key_read_sig n) =
   DM.create #_ #(key_read_sig n).ops
     (function ID_GET -> get_oracle km GET
@@ -155,7 +152,6 @@ let key_read_module (n:u32) (km:module_t (key_sig n)) : module_t (key_read_sig n
 let key_read_functor n
   : functor_t (key_sig n) (key_read_sig n)
   = fun (k:module_t (key_sig n)) -> key_read_module n k
-
 
 type key_write_labels =
   | ID_SET
@@ -170,12 +166,11 @@ let key_write_field_rels n : (l:key_write_labels -> erel (key_write_field_types 
          | ID_CSET -> arrow (lo handle ** lo (key n)) (eff_rel ((lo (key_state n))) (lo handle))
 
 let key_write_sig (n:u32) = {
-  labels = key_write_labels;
-  ops = key_write_field_types n;
-  rels = key_write_field_rels n
+    labels = key_write_labels;
+    ops = key_write_field_types n;
+    rels = key_write_field_rels n
   }
 
-#set-options "--z3rlimit 350 --max_fuel 3 --max_ifuel 4"
 let key_write_module (n:u32) (km:module_t (key_sig n)) : module_t (key_write_sig n) =
   DM.create #_ #(key_write_sig n).ops
     (function ID_SET -> get_oracle km SET
