examples/rel/Setoids.Crypto.ODH.fst
@@ -8,40 +8,38 @@ open Setoids.Crypto.KEY
 
 module DM = FStar.DependentMap
 
+#set-options "--z3rlimit 350 --max_fuel 0 --max_ifuel 0"
 let share (n:u32) = lbytes32 n
 let exponent (n:u32) = lbytes32 n
-assume val exponentiate : #n:u32 -> x:share n -> y:exponent n -> share n
-assume val generator : n:u32 -> lbytes32 n
+
+noeq
+type odh_scheme (n:u32) =
+  | OS:
+  exponentiate: (x:share n -> y:exponent n -> share n) ->
+  generator: share n ->
+  odh_scheme n
 
 let odh_state n = Map.t (share n) (option (exponent n))
 
-#set-options "--z3rlimit 350 --max_fuel 2 --max_ifuel 3"
-#set-options "--query_stats"
-/// Key state relation could be hi here.
 let gen_dh_t n =
   (lo unit)
-  ^--> eff_rel (lo (odh_state n) ** lo (key_state n)) (lo (share n))
-let gen_dh n : gen_dh_t n =
+    ^--> eff_rel (lo (odh_state n) ** lo (key_state n)) (lo (share n))
+let gen_dh n (os:odh_scheme n) : gen_dh_t n =
   fun _ ->
     combined_state  <-- get ;
     let odh_st = fst combined_state in
     let key_st = snd combined_state in
     x_exp <-- sample_multiple #(odh_state n * key_state n) n;
-    let x = exponentiate (generator n) x_exp in
+    let x = os.exponentiate os.generator x_exp in
     let s':odh_state n = Map.upd odh_st x (Some x_exp) in
     put (s',key_st) ;;
     return x
 
-/// The key_state relation should be `hi` here.
 let odh_t n =
   (lo (share n) ** lo (share n))
-  //^--> eff_rel (lo (odh_state n) ** hi (key_state n)) (lo handle)
-  ^--> eff_rel (lo (odh_state n) ** lo (key_state n)) (lo handle)
+    ^--> eff_rel (lo (odh_state n) ** lo (key_state n)) (lo handle)
 
-#reset-options
-#set-options "--z3rlimit 350 --max_fuel 2 --max_ifuel 3"
-#set-options "--query_stats"
-let odh n (key_module:module_t (key_write_sig n)) : odh_t n =
+let odh n (os:odh_scheme n) (key_module:module_t (key_write_sig n)) : odh_t n =
   fun (x,y) ->
     combined_state  <-- get ;
     let odh_st = fst combined_state in
@@ -55,7 +53,7 @@ let odh n (key_module:module_t (key_write_sig n)) : odh_t n =
         else
           (y,x)
       in
-      let k = exponentiate y x_exp in
+      let k = os.exponentiate y x_exp in
       let k_set : key_set_t n = get_oracle key_module ID_SET in
       lift_right (k_set (h, k));;
       return h
@@ -64,62 +62,55 @@ type odh_labels =
   | GEN_DH
   | ODH
 
+#set-options "--z3rlimit 350 --max_fuel 0 --max_ifuel 1"
 let odh_field_types n : odh_labels -> Type0 =
   function GEN_DH -> gen_dh_t n
          | ODH -> odh_t n
 
 let odh_field_rels n : (l:odh_labels -> erel (odh_field_types n l)) =
-  function GEN_DH -> fun _ _ -> True
-           //arrow
-           //  (lo unit)
-           //  (eff_rel (lo (odh_state n) ** lo (key_state n)) (lo (share n)))
-         | ODH -> fun _ _ -> True
-           //arrow
-           //  (lo (share n) ** lo (share n))
-           //  (eff_rel (lo (odh_state n) ** lo (key_state n)) (lo handle))
+  function GEN_DH ->
+           arrow
+             (lo unit)
+             (eff_rel (lo (odh_state n) ** lo (key_state n)) (lo (share n)))
+         | ODH ->
+           arrow
+             (lo (share n) ** lo (share n))
+             (eff_rel (lo (odh_state n) ** lo (key_state n)) (lo handle))
 
 let odh_sig (n:u32) = {
-  labels = odh_labels;
-  ops = odh_field_types n;
-  rels = odh_field_rels n
+    labels = odh_labels;
+    ops = odh_field_types n;
+    rels = odh_field_rels n
   }
 
-let odh_module (n:u32) (km:module_t (key_write_sig n)) : module_t (odh_sig n) =
+let odh_module (n:u32) (os:odh_scheme n) (km:module_t (key_write_sig n)) : module_t (odh_sig n) =
   DM.create #_ #(odh_sig n).ops
-    (function GEN_DH -> gen_dh n
-            | ODH -> odh n km)
+    (function GEN_DH -> gen_dh n os
+            | ODH -> odh n os km)
 
-let odh_functor n
+let odh_functor n os
   : functor_t (key_write_sig n) (odh_sig n)
-  = fun (k:module_t (key_write_sig n)) -> odh_module n k
+  = fun (k:module_t (key_write_sig n)) -> odh_module n os k
 
-let odh_composition n
-  : functor_t (key_sig n) (sig_prod (odh_sig n) (key_read_sig n)) =
-  functor_prod_shared_sig
-    (key_sig n)
-    (odh_sig n)
-    (key_read_sig n)
-    (comp (odh_functor n) (key_write_functor n))
+let odh_composition n os
+  : functor_t (key_sig n) (sig_prod (odh_sig n) (key_read_sig n))
+  = functor_prod_shared_sig
+    (comp (odh_functor n os) (key_write_functor n))
     (key_read_functor n)
 
-let odh0_game (n:u32)
+let odh_game0 (n:u32) os
   : functor_t (sig_unit) (sig_prod (odh_sig n) (key_read_sig n))
-  =
-  as_fun (odh_composition n (KEY.key0_module n))
+  = as_fun (odh_composition n os (KEY.key0_module n))
 
-let odh1_game (n:u32)
+let odh_game1 (n:u32) os
   : functor_t (sig_unit) (sig_prod (odh_sig n) (key_read_sig n))
-  =
-  as_fun (odh_composition n (KEY.key1_module n))
+  = as_fun (odh_composition n os (KEY.key1_module n))
 
-let odh_adversary n aes = atk (sig_unit) (sig_prod (odh_sig n) (key_read_sig n))
+let odh_adversary n = atk (sig_unit) (sig_prod (odh_sig n) (key_read_sig n))
 
 assume val odh_eps: n:u32 -> eps (sig_unit) (sig_prod (odh_sig n) (key_read_sig n))
 
 let odh_functor_rel n : per (functor_t (sig_unit) (sig_prod (odh_sig n) (key_read_sig n))) =
   fun funct_a funct_b -> True
 
-/// Questions:
-/// - What would a relation on a functor look like?
-/// - How to instantiate a hypothesis?
-let odh_assumption n = eq (odh_functor_rel n) (odh_eps n) (odh0_game n) (odh1_game n)
+//let odh_assumption n os = Perfect #(sig_unit) #(sig_prod (odh_sig n) (key_read_sig n)) #(fun _ _ -> True) (odh_game0 n os) (odh_game1 n os) ()
